examples/riscv/swap/swap_symb_transfScript.sml
@@ -49,44 +49,50 @@ open swap_symb_execTheory;
 
 val _ = new_theory "swap_symb_transf";
 
+val birs_state_ss = rewrites (type_rws ``:birs_state_t``);
+
 (* --------------------- *)
 (* Auxiliary definitions *)
 (* --------------------- *)
 
-val birs_state_ss = rewrites (type_rws ``:birs_state_t``);
-
-val bprog_tm = (fst o dest_eq o concl) bir_swap_prog_def;
-
 val init_addr_tm = (snd o dest_eq o concl) swap_init_addr_def;
 val end_addr_tm = (snd o dest_eq o concl) swap_end_addr_def;
 
-val bspec_swap_pre = ``bspec_swap_pre``;
-val bspec_swap_post = ``bspec_swap_post``;
+val bir_prog_def = bir_swap_prog_def;
+val birenvtyl_def = swap_birenvtyl_def;
+val bspec_pre_def = bspec_swap_pre_def;
+val bspec_post_def = bspec_swap_post_def;
+val prog_vars_def = swap_prog_vars_def;
 
-val birs_state_init_lbl = (snd o dest_eq o concl o EVAL)
+val symb_analysis_thm = swap_symb_analysis_thm;
+val bsysprecond_thm = swap_bsysprecond_thm;
+val prog_vars_thm = swap_prog_vars_thm;
+
+val bprog_tm = (fst o dest_eq o concl) bir_prog_def;
+val prog_vars_tm = (fst o dest_eq o concl) prog_vars_def;
+
+val birenvtyl_tm = (fst o dest_eq o concl) birenvtyl_def;
+
+val bspec_pre_tm = ``bspec_swap_pre pre_x10 pre_x11 pre_x10_mem_deref pre_x11_mem_deref``;
+val bspec_post_tm = ``bspec_swap_post pre_x10 pre_x11 pre_x10_mem_deref pre_x11_mem_deref``;
+
+val bir_state_init_lbl_tm = (snd o dest_eq o concl o EVAL)
  ``bir_block_pc (BL_Address (Imm64 ^init_addr_tm))``;
-val birs_state_end_lbl = (snd o dest_eq o concl o EVAL)
+val birs_state_end_lbl_tm = (snd o dest_eq o concl o EVAL)
  ``bir_block_pc (BL_Address (Imm64 ^end_addr_tm))``;
 
-val birs_state_init_pre =  ``birs_state_init_pre_GEN
- ^birs_state_init_lbl swap_birenvtyl
- (mk_bsysprecond
-  (bspec_swap_pre pre_x10 pre_x11 pre_x10_mem_deref pre_x11_mem_deref)
-  swap_birenvtyl)``;
+val birs_state_init_pre_tm = ``birs_state_init_pre_GEN
+ ^bir_state_init_lbl_tm ^birenvtyl_tm
+ (mk_bsysprecond ^bspec_pre_tm ^birenvtyl_tm)``;
 
-val bprog_P_tm =
- ``\x y xv yv. P_bircont swap_birenvtyl (^bspec_swap_pre x y xv yv)``;
-val bprog_Q_tm =
- ``\x y xv yv. Q_bircont (^birs_state_end_lbl) (set swap_prog_vars) (^bspec_swap_post x y xv yv)``;
+val (sys_i, L_s, Pi_f) = (symb_sound_struct_get_sysLPi_fun o concl) symb_analysis_thm;
 
 (* ------------------------------- *)
 (* BIR symbolic execution analysis *)
 (* ------------------------------- *)
 
-val (sys_i, L_s, Pi_f) = (symb_sound_struct_get_sysLPi_fun o concl) swap_symb_analysis_thm;
-
-Theorem swap_analysis_L_NOTIN_thm[local]:
-  ^birs_state_end_lbl NOTIN ^L_s
+Theorem analysis_L_NOTIN_thm[local]:
+  ^birs_state_end_lbl_tm NOTIN ^L_s
 Proof
   EVAL_TAC
 QED
@@ -96,32 +102,35 @@ QED
 (* ........................... *)
 
 Theorem birs_state_init_pre_EQ_thm[local]:
-  ^((snd o dest_comb) sys_i) = ^birs_state_init_pre
+  ^((snd o dest_comb) sys_i) = ^birs_state_init_pre_tm
 Proof
-  REWRITE_TAC [birs_state_init_pre_GEN_def, mk_bsysprecond_def, swap_bsysprecond_thm] >>
+  REWRITE_TAC [birs_state_init_pre_GEN_def, mk_bsysprecond_def, bsysprecond_thm] >>
   CONV_TAC (computeLib.RESTR_EVAL_CONV [``birs_eval_exp``] THENC birs_stepLib.birs_eval_exp_CONV)
 QED
 
-val swap_analysis_thm =
-  REWRITE_RULE [birs_state_init_pre_EQ_thm, GSYM bir_swap_prog_def] swap_symb_analysis_thm;
+val analysis_thm =
+  REWRITE_RULE [birs_state_init_pre_EQ_thm, GSYM bir_prog_def] symb_analysis_thm;
 
-Theorem swap_birenvtyl_EVAL_thm[local] =
- (REWRITE_CONV [swap_birenvtyl_def,
+Theorem birenvtyl_EVAL_thm[local] =
+ (REWRITE_CONV [birenvtyl_def,
    bir_lifting_machinesTheory.riscv_bmr_vars_EVAL,
    bir_lifting_machinesTheory.riscv_bmr_temp_vars_EVAL] THENC EVAL)
- ``swap_birenvtyl``;
+ birenvtyl_tm;
 
-val birs_state_thm = REWRITE_CONV [swap_birenvtyl_EVAL_thm] birs_state_init_pre;
+val birs_state_thm = REWRITE_CONV [birenvtyl_EVAL_thm] birs_state_init_pre_tm;
 
 (* ------ *)
 
 (* now the transfer *)
 
 val birs_symb_symbols_f_sound_prog_thm =
-  (SPEC (inst [Type`:'observation_type` |-> Type.alpha] bprog_tm) bir_symb_soundTheory.birs_symb_symbols_f_sound_thm);
+  (SPEC (inst [Type`:'observation_type` |-> Type.alpha] bprog_tm)
+        bir_symb_soundTheory.birs_symb_symbols_f_sound_thm);
 
 val birs_prop_transfer_thm =
-  (MATCH_MP symb_prop_transferTheory.symb_prop_transfer_thm birs_symb_symbols_f_sound_prog_thm);
+  (MATCH_MP 
+   symb_prop_transferTheory.symb_prop_transfer_thm
+   birs_symb_symbols_f_sound_prog_thm);
 
 (* ........................... *)
 
@@ -163,24 +172,26 @@ val type_of_bir_exp_thms =
       ] end;
 
 Theorem bprog_P_entails_thm[local]:
-  P_entails_an_interpret (bir_symb_rec_sbir ^bprog_tm)
-   (^bprog_P_tm pre_x10 pre_x11 pre_x10_mem_deref pre_x11_mem_deref)
-   (birs_symb_to_symbst ^birs_state_init_pre)
+  P_entails_an_interpret
+   (bir_symb_rec_sbir ^bprog_tm)
+   (P_bircont ^birenvtyl_tm ^bspec_pre_tm)
+   (birs_symb_to_symbst ^birs_state_init_pre_tm)
 Proof
-  ASSUME_TAC (GSYM swap_prog_vars_thm) >>
-  `swap_prog_vars = MAP PairToBVar swap_birenvtyl` by (
-    SIMP_TAC std_ss [swap_birenvtyl_def, listTheory.MAP_MAP_o, PairToBVar_BVarToPair_I_thm, listTheory.MAP_ID]
+  ASSUME_TAC (GSYM prog_vars_thm) >>
+  `^prog_vars_tm = MAP PairToBVar ^birenvtyl_tm` by (
+    SIMP_TAC std_ss [birenvtyl_def, listTheory.MAP_MAP_o, PairToBVar_BVarToPair_I_thm, listTheory.MAP_ID]
   ) >>
   POP_ASSUM (fn thm => FULL_SIMP_TAC std_ss [thm]) >>
   IMP_RES_TAC (SIMP_RULE std_ss [] P_bircont_entails_thm) >>
+
   SIMP_TAC std_ss [] >>
-  POP_ASSUM (ASSUME_TAC o Q.SPEC `bspec_swap_pre pre_x10 pre_x11 pre_x10_mem_deref pre_x11_mem_deref`) >>
-  `bir_vars_of_exp (bspec_swap_pre pre_x10 pre_x11 pre_x10_mem_deref pre_x11_mem_deref) SUBSET set (MAP PairToBVar swap_birenvtyl)` by EVAL_TAC >>
+  POP_ASSUM (ASSUME_TAC o SPEC bspec_pre_tm) >>
+  `bir_vars_of_exp ^bspec_pre_tm SUBSET set (MAP PairToBVar ^birenvtyl_tm)` by EVAL_TAC >>
   POP_ASSUM (fn thm => FULL_SIMP_TAC std_ss [thm]) >>
-  `ALL_DISTINCT (MAP FST swap_birenvtyl)` by EVAL_TAC >>
+  `ALL_DISTINCT (MAP FST ^birenvtyl_tm)` by EVAL_TAC >>
   POP_ASSUM (fn thm => FULL_SIMP_TAC std_ss [thm]) >>
-  `IS_SOME (type_of_bir_exp (bspec_swap_pre pre_x10 pre_x11 pre_x10_mem_deref pre_x11_mem_deref))` by (
-    SIMP_TAC std_ss [bspec_swap_pre_def, bspec_swap_pre_def] >>
+  `IS_SOME (type_of_bir_exp ^bspec_pre_tm)` by (
+    SIMP_TAC std_ss [bspec_pre_def] >>
     CONV_TAC (RAND_CONV (SIMP_CONV (srw_ss()) type_of_bir_exp_thms)) >>
     SIMP_TAC (std_ss++holBACore_ss) [optionTheory.option_CLAUSES]
   ) >>
@@ -194,7 +205,7 @@ QED
 (* ........................... *)
 (* proof for each end state individually: *)
 
-val sys1 = (snd o dest_eq o concl o REWRITE_CONV [swap_bsysprecond_thm]) birs_state_init_pre;
+val sys1 = (snd o dest_eq o concl o REWRITE_CONV [bsysprecond_thm]) birs_state_init_pre_tm;
 val (Pi_func, Pi_set) = dest_comb Pi_f; (* Pi_func should be exactly ``IMAGE birs_symb_to_symbst`` *)
 val sys2s = pred_setSyntax.strip_set Pi_set;
 
@@ -205,9 +216,9 @@ val strongpostcond_goals = List.map (fn sys2 => ``
     sys1 = ^sys1 ==>
     sys2 = ^sys2 ==>
     birs_symb_matchstate sys1 H' bs ==>
-    bir_eval_exp (^bspec_swap_pre pre_x10 pre_x11 pre_x10_mem_deref pre_x11_mem_deref) bs.bst_environ = SOME bir_val_true ==>
+    bir_eval_exp ^bspec_pre_tm bs.bst_environ = SOME bir_val_true ==>
     birs_symb_matchstate sys2 H' bs' ==>
-    bir_eval_exp (^bspec_swap_post pre_x10 pre_x11 pre_x10_mem_deref pre_x11_mem_deref) bs'.bst_environ = SOME bir_val_true
+    bir_eval_exp ^bspec_post_tm bs'.bst_environ = SOME bir_val_true
   ``) sys2s;
 
 (*
@@ -225,13 +236,15 @@ val Pi_thms = List.map (fn sys2 =>
     sys1 = ^sys1 ==>
     sys2 = ^sys2 ==>
     birs_symb_matchstate sys1 H bs ==>
-    ^bprog_P_tm pre_x10 pre_x11 pre_x10_mem_deref pre_x11_mem_deref (birs_symb_to_concst bs) ==>
+    P_bircont ^birenvtyl_tm ^bspec_pre_tm (birs_symb_to_concst bs) ==>
     symb_interpr_ext H' H ==>
     birs_symb_matchstate sys2 H' bs' ==>
-    ^bprog_Q_tm pre_x10 pre_x11 pre_x10_mem_deref pre_x11_mem_deref (birs_symb_to_concst bs) (birs_symb_to_concst bs')
+    Q_bircont ^birs_state_end_lbl_tm (set ^prog_vars_tm) ^bspec_post_tm
+     (birs_symb_to_concst bs) (birs_symb_to_concst bs')
   ``,
     REPEAT STRIP_TAC >>
-    Q_bircont_SOLVE3CONJS_TAC swap_prog_vars_thm >>
+    Q_bircont_SOLVE3CONJS_TAC prog_vars_thm >>
+
     `birs_symb_matchstate sys1 H' bs` by (
       METIS_TAC [bir_symb_soundTheory.birs_symb_matchstate_interpr_ext_IMP_matchstate_thm]
     ) >>
@@ -244,13 +257,15 @@ val Pi_thms = List.map (fn sys2 =>
 
 (* Q is implied by sys and Pi *)
 Theorem bprog_Pi_overapprox_Q_thm[local]:
-  Pi_overapprox_Q (bir_symb_rec_sbir ^bprog_tm)
-   (^bprog_P_tm pre_x10 pre_x11 pre_x10_mem_deref pre_x11_mem_deref)
-   (birs_symb_to_symbst ^birs_state_init_pre) ^Pi_f
-   (^bprog_Q_tm pre_x10 pre_x11 pre_x10_mem_deref pre_x11_mem_deref)
+  Pi_overapprox_Q
+   (bir_symb_rec_sbir ^bprog_tm)
+   (P_bircont ^birenvtyl_tm ^bspec_pre_tm)
+   (birs_symb_to_symbst ^birs_state_init_pre_tm) ^Pi_f
+   (Q_bircont ^birs_state_end_lbl_tm (set ^prog_vars_tm) ^bspec_post_tm)
 Proof
-  REWRITE_TAC [bir_prop_transferTheory.bir_Pi_overapprox_Q_thm, swap_bsysprecond_thm] >>
+  REWRITE_TAC [bir_prop_transferTheory.bir_Pi_overapprox_Q_thm, bsysprecond_thm] >>
   REPEAT GEN_TAC >>
+
   REWRITE_TAC [pred_setTheory.IMAGE_INSERT, pred_setTheory.IMAGE_EMPTY, pred_setTheory.IN_INSERT, pred_setTheory.NOT_IN_EMPTY] >>
   REPEAT STRIP_TAC >> (
     FULL_SIMP_TAC std_ss [] >>
@@ -269,16 +284,16 @@ val bprog_prop_holds_thm =
          birs_prop_transfer_thm
          bprog_P_entails_thm)
       bprog_Pi_overapprox_Q_thm)
-    swap_analysis_thm);
+    analysis_thm);
 
 (* ........................... *)
 (* ........................... *)
 (* ........................... *)
 
-Theorem bir_abstract_jgmt_rel_swap_thm[local] =
- (MATCH_MP
-   (MATCH_MP prop_holds_TO_abstract_jgmt_rel_thm swap_analysis_L_NOTIN_thm)
-   (REWRITE_RULE [] bprog_prop_holds_thm));
+Theorem bir_abstract_jgmt_rel_thm[local] =
+  (MATCH_MP
+    (MATCH_MP prop_holds_TO_abstract_jgmt_rel_thm analysis_L_NOTIN_thm)
+    (REWRITE_RULE [] bprog_prop_holds_thm));
 
 (* ........................... *)
 (* now manage the pre and postconditions into contract friendly "bir_exec_to_labels_triple_precond/postcond", need to change precondition to "bir_env_vars_are_initialised" for set of program variables *)
@@ -287,77 +302,76 @@ Theorem bir_abstract_jgmt_rel_swap_thm[local] =
 (* ........................... *)
 (* ........................... *)
 
-Theorem abstract_jgmt_rel_swap[local]:
+Theorem abstract_jgmt_rel_thm[local]:
  abstract_jgmt_rel (bir_ts ^bprog_tm)
   (BL_Address (Imm64 ^init_addr_tm)) {BL_Address (Imm64 ^end_addr_tm)}
-  (\st. bir_exec_to_labels_triple_precond st
-    (bspec_swap_pre pre_x10 pre_x11 pre_x10_mem_deref pre_x11_mem_deref) ^bprog_tm)
+  (\st. bir_exec_to_labels_triple_precond st ^bspec_pre_tm ^bprog_tm)
   (\st st'. bir_exec_to_labels_triple_postcond st'
     (\l. if l = BL_Address (Imm64 ^end_addr_tm)
-         then (bspec_swap_post pre_x10 pre_x11 pre_x10_mem_deref pre_x11_mem_deref)
+         then ^bspec_post_tm
          else bir_exp_false) ^bprog_tm)
 Proof
   MATCH_MP_TAC (REWRITE_RULE
    [boolTheory.AND_IMP_INTRO] abstract_jgmt_rel_bir_exec_to_labels_triple_thm) >>
   SIMP_TAC std_ss [] >>
-  Q.EXISTS_TAC `swap_birenvtyl` >>
-  
+  EXISTS_TAC birenvtyl_tm >>
+
   CONJ_TAC >- (
     (* bpre subset *)
-    REWRITE_TAC [bspec_swap_pre_def] >>
-    SIMP_TAC (std_ss++pred_setLib.PRED_SET_ss) [GSYM swap_prog_vars_thm, swap_prog_vars_def] >>    
+    REWRITE_TAC [bspec_pre_def] >>
+    SIMP_TAC (std_ss++pred_setLib.PRED_SET_ss) [GSYM prog_vars_thm, prog_vars_def] >>
     SIMP_TAC (std_ss++pred_setLib.PRED_SET_ss++holBACore_ss) [listTheory.MEM, pred_setTheory.IN_INSERT] >>
     EVAL_TAC
   ) >>
 
   CONJ_TAC >- (
     (* bpost subset *)
-    REWRITE_TAC [bspec_swap_post_def] >>
-    SIMP_TAC (std_ss++pred_setLib.PRED_SET_ss) [GSYM swap_prog_vars_thm, swap_prog_vars_def] >>
+    REWRITE_TAC [bspec_post_def] >>
+    SIMP_TAC (std_ss++pred_setLib.PRED_SET_ss) [GSYM prog_vars_thm, prog_vars_def] >>
     SIMP_TAC (std_ss++pred_setLib.PRED_SET_ss++holBACore_ss) [listTheory.MEM, pred_setTheory.IN_INSERT]
   ) >>
 
   CONJ_TAC >- (
     (* bpost is bool *)
-    REWRITE_TAC [bspec_swap_post_def] >>
+    REWRITE_TAC [bspec_post_def] >>
     SIMP_TAC (std_ss++holBACore_ss) [bir_is_bool_exp_REWRS, type_of_bir_exp_def]
   ) >>
 
   CONJ_TAC >- (
     (* ALL_DISTINCT envtyl *)
-    SIMP_TAC (std_ss++listSimps.LIST_ss) [swap_birenvtyl_EVAL_thm] >>
+    SIMP_TAC (std_ss++listSimps.LIST_ss) [birenvtyl_EVAL_thm] >>
     EVAL_TAC
   ) >>
 
   CONJ_TAC >- (
     (* envtyl = vars_of_prog *)
-    REWRITE_TAC [GSYM swap_prog_vars_thm] >>
-    SIMP_TAC std_ss [swap_birenvtyl_def, listTheory.MAP_MAP_o, PairToBVar_BVarToPair_I_thm, listTheory.MAP_ID]
+    REWRITE_TAC [GSYM prog_vars_thm] >>
+    SIMP_TAC std_ss [birenvtyl_def, listTheory.MAP_MAP_o, PairToBVar_BVarToPair_I_thm, listTheory.MAP_ID]
   ) >>
 
-  METIS_TAC [bir_abstract_jgmt_rel_swap_thm, swap_prog_vars_thm]
+  METIS_TAC [bir_abstract_jgmt_rel_thm, prog_vars_thm]
 QED
 
-Theorem bspec_cont_swap_thm[local]:
+Theorem bspec_cont_thm[local]:
  bir_cont ^bprog_tm bir_exp_true
   (BL_Address (Imm64 ^init_addr_tm)) {BL_Address (Imm64 ^end_addr_tm)} {}
-  (bspec_swap_pre pre_x10 pre_x11 pre_x10_mem_deref pre_x11_mem_deref)
+  ^bspec_pre_tm
   (\l. if l = BL_Address (Imm64 ^end_addr_tm)
-       then bspec_swap_post pre_x10 pre_x11 pre_x10_mem_deref pre_x11_mem_deref
+       then ^bspec_post_tm
        else bir_exp_false)
 Proof
  `{BL_Address (Imm64 ^end_addr_tm)} <> {}` by fs [] >>
  MP_TAC ((Q.SPECL [
   `BL_Address (Imm64 ^init_addr_tm)`,
   `{BL_Address (Imm64 ^end_addr_tm)}`,
-  `bspec_swap_pre pre_x10 pre_x11 pre_x10_mem_deref pre_x11_mem_deref`,
+  `^bspec_pre_tm`,
   `\l. if l = BL_Address (Imm64 ^end_addr_tm)
-       then (bspec_swap_post pre_x10 pre_x11 pre_x10_mem_deref pre_x11_mem_deref)
+       then ^bspec_post_tm
        else bir_exp_false`
  ] o SPEC bprog_tm o INST_TYPE [Type.alpha |-> Type`:'observation_type`])
-   abstract_jgmt_rel_bir_cont) >>
+  abstract_jgmt_rel_bir_cont) >>
  rw [] >>
- METIS_TAC [abstract_jgmt_rel_swap]
+ METIS_TAC [abstract_jgmt_rel_thm]
 QED
 
 Theorem bspec_cont_swap:
@@ -368,7 +382,7 @@ Theorem bspec_cont_swap:
        then bspec_swap_post pre_x10 pre_x11 pre_x10_mem_deref pre_x11_mem_deref
        else bir_exp_false)
 Proof
- rw [bir_swap_prog_def,bspec_cont_swap_thm]
+ rw [bir_prog_def,bspec_cont_thm]
 QED
 
 val _ = export_theory ();
